ironfleet/src/Dafny/Distributed/Protocol/RSL/FailureProof/Phase2Proof_helper.i.dfy
@@ -87,4 +87,91 @@ lemma Before2a_to_Before2a_NonLeaderAction(ts:TimestampedRslState, ts':Timestamp
     ensures pkt in ts.t_environment.sentPackets
     {}
 }
+
+
+lemma Before2b_to_After2b(ts:TimestampedRslState, ts':TimestampedRslState, opn:OperationNumber, idx:int, tios:seq<TimestampedLIoOp<NodeIdentity, RslMessage>>,
+    rs:RslState, rs':RslState, iops:seq<RslIo>
+) 
+    requires rs == UntimestampRslState(ts)
+    requires rs' == UntimestampRslState(ts')
+    requires iops == UntagLIoOpSeq(tios);
+    requires RslAssumption(ts) && RslConsistency(ts)
+    requires RslAssumption(ts') && RslConsistency(ts')
+    requires PacketsBallotInvariant(ts) && PacketsBallotInvariant(ts')
+    requires TimestampedRslNext(ts, ts')
+    requires !TimestampedRslNextEnvironment(ts, ts')
+    requires RslPerfInvariant(ts, opn)
+    requires Before_2b_Sent_Invariant(ts, opn)
+    requires TimestampedRslNextOneReplica(ts, ts', idx, tios);
+    requires LReplicaNextProcessPacket(rs.replicas[idx].replica, rs'.replicas[idx].replica, iops);
+    requires ts.t_replicas[idx].v.nextActionIndex == 0
+    requires |tios| > 0 && tios[0].LIoOpReceive? && tios[0].r.msg.v.RslMessage_2a? 
+    requires iops[0].r.src in rs.replicas[idx].replica.acceptor.constants.all.config.replica_ids
+    requires BalLeq(rs.replicas[idx].replica.acceptor.max_bal, iops[0].r.msg.bal_2a)
+    requires LeqUpperBound(iops[0].r.msg.opn_2a, rs.replicas[idx].replica.acceptor.constants.all.params.max_integer_val)
+    requires iops[0].r.msg.bal_2a == Ballot(1, 1)
+    ensures Before_2b_Sent_Invariant(ts', opn) || After_2b_Sent_Invariant(ts', opn)
+{
+    var r, r' := rs.replicas[idx].replica, rs'.replicas[idx].replica;
+    var m := iops[0].r.msg;
+    var sent_packets := ExtractSentPacketsFromIos(iops);
+    assert LAcceptorProcess2a(r.acceptor, r'.acceptor, iops[0].r, sent_packets);
+    var msg2b := RslMessage_2b(m.bal_2a, m.opn_2a, m.val_2a);
+    assert LBroadcastToEveryone(r.acceptor.constants.all.config, r.acceptor.constants.my_index, msg2b, sent_packets);
+    assert forall p | p in sent_packets :: LIoOpSend(p) in iops;
+    if m.opn_2a == opn {
+        var pkt_witness := sent_packets[0];
+        assert LIoOpSend(pkt_witness) in iops;
+        assert After_2b_Sent_Invariant(ts', opn);
+    } else {
+        assert forall p | p in sent_packets && p.msg.RslMessage_2b? :: p.msg.opn_2b != opn;
+        assert Before_2b_Sent_Invariant(ts', opn);
+    }
+}
+
+
+lemma Before2b_to_Before2b_NonReceive(ts:TimestampedRslState, ts':TimestampedRslState, opn:OperationNumber, idx:int, tios:seq<TimestampedLIoOp<NodeIdentity, RslMessage>>) 
+    requires RslAssumption(ts) && RslConsistency(ts)
+    requires RslAssumption(ts') && RslConsistency(ts')
+    requires PacketsBallotInvariant(ts) && PacketsBallotInvariant(ts')
+    requires TimestampedRslNext(ts, ts')
+    requires !TimestampedRslNextEnvironment(ts, ts')
+    requires RslPerfInvariant(ts, opn)
+    requires Before_2b_Sent_Invariant(ts, opn)
+    requires TimestampedRslNextOneReplica(ts, ts', idx, tios);
+    requires ts.t_replicas[idx].v.nextActionIndex != 0
+    ensures Before_2b_Sent_Invariant(ts', opn)
+{}
+
+lemma Before2b_to_Before2b_Receive(ts:TimestampedRslState, ts':TimestampedRslState, opn:OperationNumber, idx:int, tios:seq<TimestampedLIoOp<NodeIdentity, RslMessage>>) 
+    requires RslAssumption(ts) && RslConsistency(ts)
+    requires RslAssumption(ts') && RslConsistency(ts')
+    requires PacketsBallotInvariant(ts) && PacketsBallotInvariant(ts')
+    requires TimestampedRslNext(ts, ts')
+    requires !TimestampedRslNextEnvironment(ts, ts')
+    requires RslPerfInvariant(ts, opn)
+    requires Before_2b_Sent_Invariant(ts, opn)
+    requires TimestampedRslNextOneReplica(ts, ts', idx, tios);
+    requires ts.t_replicas[idx].v.nextActionIndex == 0
+    requires !tios[0].LIoOpTimeoutReceive?
+    requires !tios[0].r.msg.v.RslMessage_2a?
+    ensures Before_2b_Sent_Invariant(ts', opn)
+{
+    var s, s', ios := UntimestampRslState(ts), UntimestampRslState(ts'), UntagLIoOpSeq(tios);
+    var r, r' := s.replicas[idx].replica, s'.replicas[idx].replica;
+    var sent_packets := ExtractSentPacketsFromIos(ios);
+    assert forall p | p in sent_packets :: !p.msg.RslMessage_2b?;
+    forall pkt | pkt in ts'.t_environment.sentPackets && IsNew2bPacket(pkt, opn) 
+    ensures pkt in ts.t_environment.sentPackets {
+        if pkt !in ts.t_environment.sentPackets {
+            assert UntagLPacket(pkt) in sent_packets;
+            assert false;
+        }
+    }
+    forall pkt | pkt in ts'.t_environment.sentPackets && IsNew2aPacket(pkt, opn) 
+    ensures pkt in ts.t_environment.sentPackets {}
+    assert Before_2b_Sent_Invariant(ts', opn);
+}
+
+
 }
