ironfleet/src/Dafny/Distributed/Protocol/RSL/FailureProof/Phase2Proof_toplevel.i.dfy
@@ -6,7 +6,7 @@ import opened RslPhase2Proof_postFail_i
 import opened Rs2Phase2Proof_Helper
 
 
-/* Main Invariant */
+/**** MAIN INVARIANT ****/
 lemma PerfInvariantMaintained(s:TimestampedRslState, s':TimestampedRslState, req_time:Timestamp, opn:OperationNumber)
     requires RslAssumption(s) && RslAssumption(s')
     requires RslConsistency(s) && RslConsistency(s')
@@ -40,7 +40,8 @@ lemma PerfInvariantMaintained(s:TimestampedRslState, s':TimestampedRslState, req
 *                                         Lemmas                                         *
 *****************************************************************************************/
 
-/* Proof that PacketsBallotInvariant is maintained */
+/****  MAIN THEOREM ****
+* Proof that PacketsBallotInvariant is maintained */
 lemma PacketsBallotInvariant_Maintained(ts:TimestampedRslState, ts':TimestampedRslState, opn:OperationNumber) 
     requires RslAssumption(ts) && RslAssumption(ts')
     requires RslConsistency(ts') && RslConsistency(ts')
@@ -98,8 +99,48 @@ lemma Before2b_to_MaybeAfter2b(ts:TimestampedRslState, ts':TimestampedRslState, 
     requires Before_2b_Sent_Invariant(ts, opn);
     ensures Before_2b_Sent_Invariant(ts', opn) || After_2b_Sent_Invariant(ts', opn);
 {
-    // TODO
-    assume false;
-    assert Before_2b_Sent_Invariant(ts', opn) || After_2b_Sent_Invariant(ts', opn);
+    if TimestampedRslNextEnvironment(ts, ts') {
+        assert Before_2b_Sent_Invariant(ts', opn);
+        return;
+    }
+    var idx, tios:seq<TimestampedLIoOp<NodeIdentity, RslMessage>> :| TimestampedRslNextOneReplica(ts, ts', idx, tios);
+    var nextActionIndex := ts.t_replicas[idx].v.nextActionIndex;
+    if nextActionIndex != 0 {
+        Before2b_to_Before2b_NonReceive(ts, ts', opn, idx, tios);
+        return;
+    } 
+    var s, s', ios := UntimestampRslState(ts), UntimestampRslState(ts'), UntagLIoOpSeq(tios);
+    var r, r' := s.replicas[idx].replica, s'.replicas[idx].replica;
+    if ios[0].LIoOpTimeoutReceive? {
+        assert ts'.t_environment.sentPackets == ts.t_environment.sentPackets;
+        assert Before_2b_Sent_Invariant(ts', opn);
+        return;
+    }
+    // assert LReplicaNextProcessPacketWithoutReadingClock(r, r', ios);
+    var sent_packets := ExtractSentPacketsFromIos(ios);
+    if !ios[0].r.msg.RslMessage_2a? {
+        Before2b_to_Before2b_Receive(ts, ts', opn, idx, tios);
+        return;
+    }
+    // assert LReplicaNextProcess2a(r, r', ios[0].r, sent_packets);
+    var m := ios[0].r.msg;
+    if ios[0].r.src in r.acceptor.constants.all.config.replica_ids
+       && BalLeq(r.acceptor.max_bal, m.bal_2a)
+       && LeqUpperBound(m.opn_2a, r.acceptor.constants.all.params.max_integer_val)
+    {
+        if m.bal_2a == Ballot(1, 1) {
+            Before2b_to_After2b(ts, ts', opn, idx, tios, s, s', ios);
+        } else {
+            assert forall p | p in sent_packets && p.msg.RslMessage_2b? :: p.msg.bal_2b != Ballot(1, 1);
+            assert Before_2b_Sent_Invariant(ts', opn);
+        }
+    } else {
+        assert sent_packets == [];
+        reveal_ExtractSentPacketsFromIos();
+        assert forall io | io in ios :: !io.LIoOpSend?;
+        forall tio | tio in tios 
+        ensures !tio.LIoOpSend? {}
+        assert Before_2b_Sent_Invariant(ts', opn) || After_2b_Sent_Invariant(ts', opn);
+    }
 }
 }
